% \begin{subequations} 
% \begin{align}
% \mL_{x,t} &= -\alpha_x (C_t + \beta) + F_{x,t} \log(\alpha_x(C_t + \beta)) - \log(F_{x,t}!)  \\
% g_{x,t} &= -\alpha_x + F_{x,t}(C_t + \beta)^{-1} \\
% H_{x,t} &= -F_{x,t} (C_t + \beta)^{-2}
% \end{align}
% \end{subequations}
% 
% \noindent where $\mL=\sum_{x,t} \mL_{x,t}$, $\bg=\sum_x (g_{x,1}, \ldots, g_{x,T})\T$, and $\bH=\text{diag}(\sum_x H_{x,t})$.

\begin{figure}[h!]
\centering \includegraphics[width=.9\linewidth]{../figs/poisson}
\caption{Poisson} \label{fig:poiss}
\end{figure}
