\paragraph{Model}

\begin{align}
	\bF_{x,t} \sim \text{Poisson}(\alpha_x (C_t + \beta))
\end{align}

\paragraph{Inference}

\begin{subequations} 
\begin{align}
\mL_{x,t} &= -\alpha_x (C_t + \beta) + F_{x,t} \log(\alpha_x(C_t + \beta)) - \log(F_{x,t}!)  \\
g_{x,t} &= -\alpha_x + F_{x,t}(C_t + \beta)^{-1} \\
H_{x,t} &= -F_{x,t} (C_t + \beta)^{-2}
\end{align}
\end{subequations}

\noindent where $\mL=\sum_{x,t} \mL_{x,t}$, $\bg=\sum_x (g_{x,1}, \ldots, g_{x,T})\T$, and $\bH=\text{diag}(\sum_x H_{x,t})$.